execution/examples/BATCommon.v
@@ -1,0 +1,435 @@
+From Coq Require Import List
+                        ZArith_base
+                        Lia.
+Import ListNotations.
+From ConCert Require Import RecordUpdate
+                            Extras
+                            Containers
+                            Automation
+                            Serializable
+                            Blockchain.
+Import RecordSetNotations.
+Require EIP20Token.
+
+
+Section BATCommon.
+
+Context {BaseTypes : ChainBase}.
+Set Primitive Projections.
+Set Nonrecursive Elimination Schemes.
+
+Definition TokenValue := EIP20Token.TokenValue.
+
+Inductive Msg :=
+  (* Message types from the EIP20/ERC20 Standard Token: *)
+  | tokenMsg : EIP20Token.Msg -> Msg
+  (* Message types specific for BAT: *)
+  (* create_tokens acceps the currency of the chain and converts it to BAT according to the pre-specified exchange rate *)
+  | create_tokens : Msg
+  (* finalize ends the funding period and sends the chain currency home to the pre-specified fund deposit address. Only callable by this address *)
+  | finalize : Msg
+  (* Allows contributors to recover their ether in the case of a failed funding campaign. *)
+  | refund : Msg.
+
+Record State :=
+  build_state {
+    (* State from EIP20Token: *)
+    token_state       : EIP20Token.State;
+    (* State for BAT: *)
+    initSupply        : N;
+    fundDeposit    		: Address;
+    batFundDeposit 		: Address;
+    isFinalized    		: bool;
+    fundingStart   		: nat;
+    fundingEnd	 	 		: nat;
+    tokenExchangeRate : N;
+    tokenCreationCap 	: N;
+    tokenCreationMin 	: N;
+  }.
+
+Record Setup :=
+  build_setup {
+    _batFund						: N;
+    _fundDeposit 				: Address;
+    _batFundDeposit 		: Address;
+    _fundingStart	  		: nat;
+    _fundingEnd					: nat;
+    (* In the reference implementation, the fields below are constants, but we allow setting them at initialisation, in order to test out different values. *)
+    _tokenExchangeRate  : N;
+    _tokenCreationCap 	: N;
+    _tokenCreationMin 	: N;
+  }.
+
+MetaCoq Run (make_setters State).
+MetaCoq Run (make_setters Setup).
+
+Section Serialization.
+
+Global Instance setup_serializable : Serializable Setup :=
+  Derive Serializable Setup_rect <build_setup>.
+
+Global Instance msg_serializable : Serializable Msg :=
+  Derive Serializable Msg_rect <tokenMsg, create_tokens, finalize, refund>.
+
+Global Instance state_serializable : Serializable State :=
+  Derive Serializable State_rect <build_state>.
+
+End Serialization.
+
+Definition returnIf (cond : bool) := if cond then None else Some tt.
+Definition total_supply (state : State) := state.(token_state).(EIP20Token.total_supply).
+Definition balances (state : State) := state.(token_state).(EIP20Token.balances).
+Definition allowances (state : State) := state.(token_state).(EIP20Token.allowances).
+Definition transfer t a := tokenMsg (EIP20Token.transfer t a).
+Definition transfer_from f t a := tokenMsg (EIP20Token.transfer_from f t a).
+Definition approve d a := tokenMsg (EIP20Token.approve d a).
+
+Definition serializeMsg msg := (@serialize Msg _) msg.
+Definition serializeState state := (@serialize State _) state.
+Definition serializeSetup setup := (@serialize Setup _) setup.
+
+Global Coercion serializeMsg : Msg >-> SerializedValue.
+Global Coercion serializeState : State >-> SerializedValue.
+Global Coercion serializeSetup : Setup >-> SerializedValue.
+
+Definition finalize_act cstate caddr : Action :=
+  build_act (fundDeposit cstate) (act_call caddr 0%Z finalize).
+
+Definition deploy_act setup contract from : Action :=
+  build_act from (act_deploy 0%Z contract setup).
+
+(* Utility definitions and lemmas *)
+Open Scope N_scope.
+(* Stronger version of N.mod_le.
+   N.mod_le requires that b <> 0, however
+   it is possible to prove the same without
+   that assumption *)
+Lemma N_mod_le : forall a b, a mod b <= a.
+Proof.
+  intros a b. destruct (N.le_gt_cases b a).
+  - unfold N.modulo. unfold N.div_eucl.
+    destruct a.
+    + apply N.le_0_l.
+    + destruct b.
+      * apply N.le_refl.
+      * apply N.le_trans with (N.pos p0); auto.
+        apply N.lt_le_incl.
+        apply N.pos_div_eucl_remainder. lia.
+  - rewrite N.lt_eq_cases; right.
+    apply N.mod_small; auto.
+Qed.
+
+Lemma N_add_le : forall n m p,
+  n <= m -> n <= p + m.
+Proof.
+ lia.
+Qed.
+
+Lemma N_le_add_distr : forall n m p,
+ n + m <= p -> n <= p.
+Proof.
+  lia.
+Qed.
+
+Lemma N_le_sub : forall n m p,
+  p <= m ->
+  n <= m - p ->
+  n + p <= m.
+Proof.
+  lia.
+Qed.
+
+Lemma N_div_mul_le : forall n m,
+  (n / m) * m <= n.
+Proof.
+  intros.
+  rewrite N.div_mod' with (b:= m).
+  rewrite N.mul_comm.
+  apply N.le_add_r.
+Qed.
+
+Lemma N_le_div_mul : forall n m,
+  m <> 0 ->
+  n - m <= (n / m) * m.
+Proof.
+  intros.
+  eapply N.add_le_mono_r.
+  rewrite N.mul_comm.
+  rewrite <- N.div_mod' with (b:= m).
+  apply N_le_sub.
+  - apply N.mod_le; auto.
+  - apply N.sub_le_mono_l.
+    apply N.lt_le_incl.
+    apply N.mod_lt; auto.
+Qed.
+
+Lemma sumN_in_le : forall {A} x (f : A -> N) l,
+  In x l -> f x <= EIP20Token.sumN f l.
+Proof.
+  intros.
+  induction l.
+  - inversion H.
+  - apply in_inv in H as [H | H].
+    + cbn. subst.
+      rewrite N.add_comm.
+      apply N_add_le, N.le_refl.
+    + cbn.
+      now apply N_add_le, IHl.
+Qed.
+
+(* The balance of a single account is always less than
+   or equal to the sum of all balances *)
+Lemma balance_le_sum_balances : forall addr state,
+  with_default 0 (FMap.find addr (balances state)) <= EIP20Token.sum_balances (token_state state).
+Proof.
+  intros.
+  unfold EIP20Token.sum_balances.
+  destruct (FMap.find addr (balances state)) eqn:balance.
+  - cbn. apply FMap.In_elements in balance.
+    apply sumN_in_le with (f:= fun '(_, v) => v) in balance.
+    now eapply N.le_trans.
+  - apply N.le_0_l.
+Qed.
+
+(* sumZ over balances is always positive *)
+Lemma sum_balances_positive : forall bstate accounts,
+  reachable bstate ->
+  (0 <= sumZ (fun acc : Address => env_account_balances bstate acc) accounts)%Z.
+Proof.
+  intros.
+  induction accounts; cbn.
+  - lia.
+  - apply Z.add_nonneg_nonneg; auto.
+    apply Z.ge_le.
+    now apply account_balance_nonnegative.
+Qed.
+
+Lemma sumZ_le : forall {A} l (f g : A -> Z),
+  (forall a, In a l -> f a <= g a)%Z ->
+  (sumZ f l <= sumZ g l)%Z.
+Proof.
+  intros.
+  induction l.
+  - apply Z.le_refl.
+  - cbn.
+    apply Z.add_le_mono.
+    + apply H, in_eq.
+    + apply IHl.
+      intros.
+      now apply H, in_cons.
+Qed.
+
+(* Sums balances of a list of accounts *)
+Definition total_balance bstate accounts : Amount :=
+  let account_balance := env_account_balances bstate in
+    sumZ (fun acc => account_balance acc) accounts.
+
+(* Sum of balances is always positive *)
+Lemma total_balance_positive : forall bstate accounts,
+  reachable bstate -> 
+  (0 <= total_balance bstate accounts)%Z.
+Proof.
+  intros.
+  unfold total_balance.
+  now apply sum_balances_positive.
+Qed.
+
+Lemma total_balance_distr : forall state h t x,
+  reachable state ->
+  Z.to_N (total_balance state (h :: t)) * x =
+    Z.to_N (env_account_balances state h) * x +
+    Z.to_N (total_balance state t) * x.
+Proof.
+  intros.
+  cbn.
+  rewrite Z2N.inj_add.
+  - now rewrite N.mul_add_distr_r.
+  - apply Z.ge_le.
+    now apply account_balance_nonnegative.
+  - now apply sum_balances_positive.
+Qed.
+
+(* total balance equality if all accounts have equal balance *)
+Lemma total_balance_eq : forall env1 env2 accounts,
+  (forall a, In a accounts -> env_account_balances env1 a = env_account_balances env2 a) ->
+    total_balance env1 accounts = total_balance env2 accounts.
+Proof.
+  intros.
+  unfold total_balance.
+  rewrite sumZ_map_id.
+  setoid_rewrite sumZ_map_id at 2.
+  f_equal.
+  now apply map_ext_in.
+Qed.
+
+Lemma total_balance_le : forall env1 env2 accounts,
+  (forall a, In a accounts -> env_account_balances env1 a <= env_account_balances env2 a)%Z ->
+    (total_balance env1 accounts <= total_balance env2 accounts)%Z.
+Proof.
+  intros.
+  now apply sumZ_le.
+Qed.
+
+(* pending usage is the total balance that an account has allocated
+   in the pending actions.
+   Does not count actions with negative amount and caps the usage
+   at the balance limit of the account. *)
+Definition pending_usage bstate account : Amount :=
+  Z.min (sumZ (fun act => if address_eqb act.(act_from) account
+                         then Z.max 0 (act_amount act) 
+                         else 0%Z) bstate.(chain_state_queue))
+        (env_account_balances bstate account).
+
+(* Spendable blance is the balance of an account minus their pending
+   usage, i.e. the minimum amount that the account is guaranteed to have
+   available for usage next block. *)
+Definition spendable_balance (bstate : ChainState) accounts : Amount :=
+  let account_balance := env_account_balances bstate in
+    sumZ (fun acc => account_balance acc - pending_usage bstate acc)%Z accounts.
+
+(* Spendable balance is equal to total balance if there is no
+   pending actions left in the current block. *)
+Lemma spendable_eq_total_balance : forall bstate accounts,
+  reachable bstate ->
+  chain_state_queue bstate = [] ->
+  spendable_balance bstate accounts = total_balance bstate accounts.
+Proof.
+  intros bstate accounts reach queue.
+  unfold spendable_balance, total_balance, pending_usage.
+  rewrite queue. cbn.
+  rewrite sumZ_map_id.
+  setoid_rewrite sumZ_map_id at 2.
+  f_equal.
+  apply map_ext_in.
+  intros.
+  rewrite Z.min_l, Z.sub_0_r; auto.
+  apply Z.ge_le.
+  now apply account_balance_nonnegative.
+Qed.
+
+(* Spendable balance cannot decrease when consuming or discarding
+   actions from the queue. *)
+Lemma spendable_consume_act : forall (bstate1 bstate2 : ChainState) accounts act acts,
+  (env_account_balances bstate1 act.(act_from) <= env_account_balances bstate2 act.(act_from) + (Z.max 0 (act_amount act)))%Z ->
+  (forall a, In a accounts -> a <> act.(act_from) -> env_account_balances bstate1 a <= env_account_balances bstate2 a)%Z ->
+  chain_state_queue bstate1 = act :: acts ->
+  chain_state_queue bstate2 = acts ->
+  (spendable_balance bstate1 accounts <= spendable_balance bstate2 accounts)%Z.
+Proof.
+  intros bstate_from bstate_to accounts act acts
+         act_balance other_balances queue_from queue_to.
+  induction accounts.
+  - apply Z.le_refl.
+  - cbn.
+    apply Z.add_le_mono.
+    + destruct (address_eqdec a (act_from act));
+        unfold pending_usage; rewrite queue_from, queue_to; cbn.
+      * subst.
+        rewrite address_eq_refl.
+        lia.
+      * rewrite address_eq_ne; auto.
+        apply other_balances in n; try apply in_eq.
+        lia.
+    + apply IHaccounts.
+      intros.
+      apply other_balances; eauto.
+      now apply in_cons.
+Qed.
+
+(* Spendable balance is always positive *)
+Lemma spendable_balance_positive : forall bstate accounts,
+  reachable bstate ->
+  (0 <= spendable_balance bstate accounts)%Z.
+Proof.
+  intros.
+  unfold spendable_balance.
+  induction accounts.
+  - apply Z.le_refl.
+  - cbn.
+    apply Ztac.add_le;
+    unfold pending_usage in *;
+    lia.
+Qed.
+
+(* Function that generated create_token actions.
+   Will keep generating action untill all accounts given have been emptied of balance
+   or the token goal is hit. Also ensures that we do not hit the token creation cap
+   by only creation just enough to go over the token goal. *)
+Fixpoint create_token_acts (env : Environment) caddr accounts tokens_left exchange_rate:=
+  let create_tokens_act sender amount := build_act sender (act_call caddr amount create_tokens) in
+    match accounts with
+    | [] => []
+    | acc :: accounts' =>
+      (* Dont produce any action for this account if tokens_left = 0 *)
+      if 0 <? tokens_left
+      then
+        let amount := 1 + ((tokens_left / exchange_rate)) in
+        (* Choose the minimum amount of balance needed to hit tokens_left = 0 or all balance
+            if the account does not have enough balance to hit goal *)
+        let amount := N.min amount (Z.to_N (env_account_balances env acc)) in
+          (create_tokens_act acc (Z.of_N amount)) ::
+          create_token_acts env caddr accounts' (N.sub tokens_left (amount * exchange_rate)) exchange_rate
+      else
+        create_token_acts env caddr accounts' tokens_left exchange_rate
+    end.
+
+Lemma create_token_acts_cons : forall caddr env acc accounts tokens_left exchange_rate,
+  let create_tokens_act sender amount := build_act sender (act_call caddr amount create_tokens) in
+  let amount' := 1 + ((tokens_left / exchange_rate)) in
+  let amount := N.min amount' (Z.to_N (env_account_balances env acc)) in
+  let act := create_tokens_act acc (Z.of_N amount) in
+  0 < tokens_left->
+  create_token_acts env caddr (acc :: accounts) tokens_left exchange_rate =
+  act :: (create_token_acts env caddr accounts (tokens_left - (amount * exchange_rate))) exchange_rate.
+Proof.
+  intros.
+  cbn.
+  destruct_match eqn:Htokens_left; eauto.
+  now apply N.ltb_nlt in Htokens_left.
+Qed.
+
+Lemma create_token_acts_eq : forall caddr env1 env2 accounts tokens_left exchange_rate,
+  (forall a, In a accounts -> env_account_balances env1 a = env_account_balances env2 a) ->
+    create_token_acts env1 caddr accounts tokens_left exchange_rate =
+    create_token_acts env2 caddr accounts tokens_left exchange_rate.
+Proof.
+  induction accounts; intros.
+  - reflexivity.
+  - cbn.
+    rewrite H by apply in_eq.
+    now do 2 rewrite <- IHaccounts by (intros; now apply H, in_cons).
+Qed.
+
+(* All actions produced by create_token_acts are from accounts *)
+Lemma create_token_acts_is_account : forall caddr env accounts tokens_left exchange_rate,
+  Forall (fun acc : Address => address_is_contract acc = false) accounts ->
+    (forall x : Action, In x (create_token_acts env caddr accounts tokens_left exchange_rate) -> act_is_from_account x).
+Proof.
+  induction accounts; intros ? ? is_address act HIn.
+  - inversion HIn.
+  - cbn in HIn.
+    apply list.Forall_cons in is_address as [is_address is_address'].
+    destruct_match in HIn. destruct HIn; subst.
+    all: eauto.
+Qed.
+Close Scope N_scope.
+
+End BATCommon.
+
+(* ------------------- Definitions from EIP20Token ------------------- *)
+Notation isSome := EIP20Token.isSome.
+Notation sumN := EIP20Token.sumN.
+Notation "'sum_balances' s" := (EIP20Token.sum_balances (token_state s)) (at level 60).
+Notation get_allowance := EIP20Token.get_allowance.
+Notation transfer_balance_update_correct := EIP20Token.transfer_balance_update_correct.
+Notation transfer_from_allowances_update_correct := EIP20Token.transfer_from_allowances_update_correct.
+Notation approve_allowance_update_correct := EIP20Token.approve_allowance_update_correct.
+
+Existing Instance EIP20Token.sumN_perm_proper.
+
+Ltac returnIf H :=
+  let G := fresh "G" in
+    unfold returnIf in H;
+    destruct_match eqn:G in H; try congruence;
+    clear H;
+    rename G into H.
